theories/strongInduction.v
@@ -1,0 +1,44 @@
+(*Adapted from https://github.com/tchajed/strong-induction/blob/master/StrongInduction.v*)
+
+Require Import PeanoNat.
+Require Import ZArith Psatz.
+
+Section StrongInduction.
+
+  Variable P:nat -> Set.
+
+  (** The stronger inductive hypothesis given in strong induction. The standard
+  [nat ] induction principle provides only n = pred m, with [P 0] required
+  separately. *)
+  Hypothesis IH : forall m, (forall n, n < m -> P n) -> P m.
+
+
+  Hint Resolve le_S_n.
+
+  (** * Strengthen the induction hypothesis. *)
+
+  Local Lemma strong_induction_all : forall n,
+      (forall m, m <= n -> P m).
+  Proof.
+    intro n.
+    induction n.
+    - intros m H.
+      rewrite Nat.le_0_r in H.
+      apply IH.
+      intros n H0.
+      subst.
+      apply Nat.nlt_0_r in H0.
+      contradiction.
+    - intros m H.
+      apply IH.
+      intros n0 H0.
+      apply IHn.
+      lia.
+  Defined.
+
+  Theorem strong_induction : forall n, P n.
+  Proof.
+    eauto using strong_induction_all.
+  Defined.
+
+End StrongInduction.
